src/Result.v
@@ -1,0 +1,130 @@
+(** Result.
+  This file describes the [result] monad. **)
+
+(* Copyright © 2018 Martin Bodin
+
+  This program is free software; you can redistribute it and/or modify
+  it under the terms of the GNU General Public License as published by
+  the Free Software Foundation; either version 2 of the License, or
+  (at your option) any later version.
+
+  This program is distributed in the hope that it will be useful,
+  but WITHOUT ANY WARRANTY; without even the implied warranty of
+  MERCHANTABILITY or FITNESS FOR A PARTICULAR PURPOSE.  See the
+  GNU General Public License for more details.
+
+  You should have received a copy of the GNU General Public License
+  along with this program; if not, write to the Free Software
+  Foundation, Inc., 51 Franklin St, Fifth Floor, Boston, MA  02110-1301 USA *)
+
+Set Implicit Arguments.
+Require Import Rinternals State InternalTypes Globals.
+
+
+(** * Monadic Type **)
+
+(** A monad type for results. **)
+Inductive rresult (A : Type) :=
+  | rresult_success : A -> state -> rresult A (** The program resulted in this state with this result. **)
+  | rresult_longjump : nat -> context_type -> state -> rresult A (** The program yielded a call to [LONGJMP] with these arguments. **)
+  | rresult_error_stack : list string -> string -> state -> rresult A (** The program resulted in the following error (not meant to be caught). **)
+  | rresult_impossible_stack : list string -> string -> state -> rresult A (** This result should never happen. We provide a string and a call stack to help debugging. **)
+  | rresult_not_implemented_stack : list string -> string -> rresult A (** The result relies on a feature not yet implemented. **)
+  | rresult_bottom : state -> rresult A (** We went out of fuel during the computation. **)
+  .
+Arguments rresult_success [A].
+Arguments rresult_longjump [A].
+Arguments rresult_error_stack [A].
+Arguments rresult_impossible_stack [A].
+Arguments rresult_not_implemented_stack [A].
+Arguments rresult_bottom {A}.
+
+(** We wrap [rresult] in a state monad. **)
+Definition result A := Globals -> state -> rresult A.
+
+
+Definition result_success : forall A, A -> result A :=
+  fun _ a _ => rresult_success a.
+Arguments result_success [A].
+
+Definition result_longjump (A : Type) : nat -> context_type -> result A :=
+  fun i ct _ => rresult_longjump i ct.
+Arguments result_longjump [A].
+
+Definition result_error (A : Type) msg : result A :=
+  fun _ => rresult_error_stack nil msg.
+Arguments result_error [A].
+
+Definition result_impossible (A : Type) msg : result A :=
+  fun _ => rresult_impossible_stack nil msg.
+Arguments result_impossible [A].
+
+Definition result_not_implemented (A : Type) msg : result A :=
+  fun _ S => rresult_not_implemented_stack nil msg.
+Arguments result_not_implemented [A].
+
+Definition result_bottom : forall A, result A :=
+  fun _ _ => rresult_bottom.
+Arguments result_bottom {A}.
+
+Global Instance result_Inhab : forall A, Inhab (result A) :=
+  fun _ => prove_Inhab (result_impossible "[arbitrary]").
+
+
+(** A precision about [result_not_implemented] and [result_error]:
+  if the C source code of R throw a not-implemented error, we consider
+  this as an error thrown in the original interpreter and use the
+  constructor [result_error].
+  We only throw [result_not_implemented] when our Coq code has not
+  implemented a behaviour of R.
+  The construct [result_error] thus models the errors thrown by the
+  R program. **)
+
+(** The difference between [result_error] and [result_impossible] is
+  that [result_error] is thrown when the R interpreter throws an error
+  (usally using the [error] C function), and [result_impossible] is
+  thrown when R does not throw an error, but we know for sure that such
+  a case can never happen, or such a case would lead an undefined
+  behaviour in the original program. Typically because the C program accepts
+  an impossible case to be missing, but that Coq does not recognise this
+  case to be impossible. So if there is a possible case in which Coq
+  must return something, but that the R interpreter in C does not cover
+  this case (for instance by writting [e->type] without checking whether
+  [e] actually maps to a valid expression), the Coq interpreter will
+  return [result_impossible]. **)
+
+
+(** * [FUNTAB] **)
+
+(** This section defines the [FUNTAB] structure, which is used to store
+  primitive and internal functions, as well as some constructs to
+  evaluate it. Most of these constructs can be found in
+  include/Defn.h. **)
+
+(** Following GNU R, all functions in the array [R_FunTab] have the same type: they take four SEXP
+  and return an SEXP.
+  The four SEXP respectively correspond to the call, op, args, and rho parameters of each functions.
+  The most important is args, which is an R list of arguments. **)
+Definition function_code :=
+  SEXP -> (** call **)
+  SEXP -> (** op **)
+  SEXP -> (** args **)
+  SEXP -> (** rho **)
+  result SEXP.
+
+(** [FUNTAB] **)
+Record funtab_cell := make_funtab_cell {
+    fun_name : string ;
+    fun_cfun : function_code ;
+    fun_code : int ; (** The number stored here can be quite large. We thus use [int] instead of [nat] here. **)
+    fun_eval : funtab_eval_arg ;
+    fun_arity : int ;
+    fun_gram : PPinfo
+  }.
+
+Instance funtab_cell_Inhab : Inhab funtab_cell.
+  apply prove_Inhab. constructors; apply arbitrary.
+Qed.
+
+Definition funtab := ArrayList.array funtab_cell.
+
